theories/Compositional_Structures/Basic_Modules/Borda_Module_Ref.thy
@@ -48,24 +48,24 @@ qed
 
 
 lemma borda_score_evalf_rel:
-  fixes A:: "'a set"
-  assumes 
-    fina: "finite A"
-  shows "((\<lambda> x. borda_score_mon x A), (\<lambda> x p. RETURN ( borda_score x A p )))
+  shows "(borda_score_mon, (\<lambda> x A p. RETURN ( borda_score x A p )))
     \<in> evalf_rel"
   apply (refine_vcg)
-proof (clarify, unfold borda_score_mon.simps, rename_tac x' x pl pr)
+proof (clarify, unfold borda_score_mon.simps, rename_tac  x' x A' A pl pr)
+  fix A' A :: "'a set"
   fix x :: 'a
   fix pl :: "'a Profile_List"
   fix pr :: "'a Profile"
+  assume arel: "(A', A) \<in> \<langle>Id\<rangle>fset_rel"
   assume prel: "(pl, pr) \<in> profile_rel"
-  from this fina 
-  show " FOREACH A (\<lambda>y sc. prefer_count_monadic_imp pl x y 
-        \<bind> (\<lambda>pcx. RETURN (sc + pcx))) 0
-        \<le> SPEC (\<lambda>c. (c, borda_score x A pr) \<in> nat_rel)"
+  from arel have aeq: "A' = A" by (auto simp add: fset_rel_def in_br_conv)
+  from arel have fina: "finite A'" by (auto simp add: fset_rel_def in_br_conv)
+  from this 
+  show "FOREACH A' (\<lambda>y sc. prefer_count_monadic_imp pl x y \<bind> (\<lambda>pcx. RETURN (sc + pcx))) 0
+       \<le> SPEC (\<lambda>c. (c, borda_score x A pr) \<in> nat_rel)"
   proof (refine_vcg FOREACH_rule[where I = 
         "(\<lambda>it sc. sc = (\<Sum> y \<in> (A - it). (prefer_count pr x y)))"],
-      clarsimp_all simp add: fina simp del:  prefer_count.simps)
+      clarsimp_all simp add: fina aeq simp del:  prefer_count.simps)
     fix xa :: 'a
     fix it :: "'a set"
     assume xit: "xa \<in> it"
@@ -73,7 +73,7 @@ proof (clarify, unfold borda_score_mon.simps, rename_tac x' x pl pr)
     from prel have pcref: "prefer_count_monadic_imp pl x xa 
         \<le> SPEC (\<lambda> pcxa. pcxa = prefer_count pr x xa)" 
     using prefer_count_monadic_imp_correct by fastforce
-    from fina itA xit have "sum (prefer_count pr x) (A - it) + (prefer_count pr x xa)
+    from fina itA xit aeq have "sum (prefer_count pr x) (A - it) + (prefer_count pr x xa)
       = sum (prefer_count pr x) (A - (it - {xa}))"
       by (metis Diff_iff ab_semigroup_add_class.add.commute finite_Diff it_step_insert_iff sum.insert)
     from pcref this show "prefer_count_monadic_imp pl x xa
@@ -83,8 +83,32 @@ proof (clarify, unfold borda_score_mon.simps, rename_tac x' x pl pr)
   qed
 qed
 
-context voting_session
-begin
+
+
+locale sepvs = voting_session 
+
+begin                                       
+
+lemma bcseptest:
+  shows "(borda_monadic, (\<lambda> A p. RETURN (borda A p))) \<in>
+    (alts_set_rel) \<rightarrow> profile_rel \<rightarrow> \<langle>Id\<rangle>nres_rel"
+  apply (refine_vcg)
+proof (unfold borda_monadic_def borda.simps, rename_tac Al' Al ppl ppr)
+  fix Al' Al :: "'a set"
+  fix pl :: "'a Profile_List"
+  fix pr :: "'a Profile"
+  assume "(pl, pr) \<in> profile_rel"
+  assume arel: "(Al', Al) \<in> alts_set_rel"
+  from this have Alid: "(Al', Al) \<in> Id"
+    by (simp add: in_br_conv)
+  from arel have fina: "finite Al'"   by (simp add: in_br_conv)
+  from Alid have Ale: "Al' = Al" by auto
+  from this  have "pre_compute_scores borda_score_mon Al' pl 
+          \<le> SPEC (\<lambda> map. map = pre_computed_map borda_score Al' pr)"
+  using fina borda_score_evalf_rel[where A = Al']
+      compute_scores_correct[THEN nres_relD, THEN refine_IdD]
+  by fastforce 
+
 
 theorem borda_ref_correct:
   shows "borda_monadic A pl \<le> SPEC (\<lambda> res. res = borda A pr)"
@@ -104,7 +128,27 @@ proof (unfold borda_monadic_def borda.simps)
     by fastforce
 qed
 
-end
+(*lemma bcseptest:
+  shows "(borda_monadic, (\<lambda> A p. RETURN (borda A p))) \<in>
+    (\<langle>Id\<rangle>set_rel O br (\<lambda>x. x) finite) \<rightarrow> profile_rel \<rightarrow>  \<langle>\<langle>Id\<rangle>set_rel \<times>\<^sub>r \<langle>Id\<rangle>set_rel \<times>\<^sub>r \<langle>Id\<rangle>set_rel\<rangle>nres_rel"
+  apply (refine_vcg)
+proof (unfold borda_monadic_def borda.simps, rename_tac Al' Al ppl ppr)
+*)
+
+
+
+
+
+
+abbreviation "profile_impl_assn \<equiv> (list_assn (array_assn nat_assn))"
+
+abbreviation "alts_set_impl_assn \<equiv> (hs.assn nat_assn)"
+
+
+definition "alts_set_assn 
+    \<equiv> hr_comp alts_set_impl_assn alts_set_rel"
+
+find_theorems id_assn
 
 sepref_definition borda_elim_sepref is
   "uncurry borda_monadic":: 
@@ -124,8 +168,11 @@ sepref_definition borda_elim_sepref is
   apply (rewrite in "_ \<bind> (\<lambda>(rej, def). if def = {} then RETURN (_, _, rej) else RETURN (\<hole>, rej, def))" hs.fold_custom_empty)
 
   apply sepref_dbg_keep
+
   done
 
 
+thm borda_elim_sepref.refine
 
+end
 end
